Merge branch 'master' of ssh://github.mit.edu/plv/fiat

src/Parsers/Refinement/IndexedAndAtMostOneNonTerminalReflective.v
@@ -1,14 +1,30 @@
-(** * Reflective helpers for simply-typed interface of the parser *)
-Require Import Coq.Lists.List Coq.Strings.String.
-Require Import ADTSynthesis.Parsers.ContextFreeGrammar.
-Require Import ADTSynthesis.Parsers.ContextFreeGrammarProperties.
-Require Import ADTSynthesis.Parsers.ContextFreeGrammarEquality.
+(** First step of a splitter refinement; indexed representation, and handle all rules with at most one nonterminal; leave a reflective goal *)
+Require Import Coq.Strings.String Coq.Arith.Lt Coq.Lists.List.
+Require Import Coq.Numbers.Natural.Peano.NPeano.
+Require Import ADTSynthesis.Parsers.StringLike.Core.
 Require Import ADTSynthesis.Parsers.ParserInterface.
-Require Import ADTSynthesis.Parsers.Refinement.IndexedAndAtMostOneNonTerminal.
-Require Import ADTSynthesis.Computation.Core.
+Require Import ADTSynthesis.Parsers.ParserADTSpecification.
+Require Import ADTSynthesis.Parsers.StringLike.Properties.
+Require Import ADTSynthesis.Parsers.StringLike.String.
+Require Import ADTSynthesis.Parsers.ContextFreeGrammarEquality.
+Require Import ADTNotation.BuildADT ADTNotation.BuildADTSig.
+Require Import ADT.ComputationalADT.
 Require Import ADTSynthesis.Common ADTSynthesis.Common.Equality.
+Require Import ADTSynthesis.ADTRefinement.
+Require Import ADTSynthesis.Common.StringBound ADTSynthesis.Common.ilist.
+Require Import ADTRefinement.BuildADTRefinements.HoneRepresentation.
+Require Import ADTSynthesis.Common.IterateBoundedIndex.
+Require Import ADTSynthesis.Common.List.FlattenList.
+Require Import ADTSynthesis.Common.List.ListFacts.
+Require Import ADTSynthesis.ADTRefinement.GeneralBuildADTRefinements.
+Require Import ADTSynthesis.Computation.SetoidMorphisms.
 
 Set Implicit Arguments.
+
+Local Open Scope list_scope.
+Local Open Scope ADTSig_scope.
+Local Open Scope ADT_scope.
+Local Open Scope string_scope.
 
 Fixpoint tails {A} (ls : list A) : list (list A)
   := match ls with
@@ -22,8 +38,8 @@ Definition forall_reachable_productions {Char} (G : grammar Char) {T} (f : produ
   := fold_right
        f
        init
-       (flatten1
-          (flatten1
+       (flatten
+          (flatten
              (map
                 (fun nt =>
                    (map
@@ -31,146 +47,449 @@ Definition forall_reachable_productions {Char} (G : grammar Char) {T} (f : produ
                       (Lookup G nt)))
                 (Valid_nonterminals G)))).
 
-Global Arguments forall_reachable_productions / .
+Lemma forall_reachable_productions_impl_helper {Char} (G : grammar Char) (Pnil : Prop) (P1 P2 : _ -> _ -> Prop)
+: forall_reachable_productions G (fun p H => (match p with
+                                                | [] => True
+                                                | x::xs => P1 x xs
+                                              end -> match p with
+                                                       | [] => Pnil
+                                                       | x::xs => P2 x xs
+                                                     end)
+                                             /\ H) True
+  -> forall_reachable_productions G (fun p H => match p with
+                                                  | [] => Pnil
+                                                  | x::xs => P1 x xs -> P2 x xs
+                                                end /\ H) True.
+Proof.
+  unfold forall_reachable_productions.
+  match goal with
+    | [ |- _ -> fold_right _ _ ?ls ] => induction ls; simpl; trivial; []
+  end.
+  intros [H0 H1]; split; eauto.
+  match goal with
+    | [ |- match ?e with _ => _ end ] => destruct a; eauto
+  end.
+Qed.
 
-Section interface.
+Lemma forall_reachable_productions_helper {Char Char_beq}
+      (Char_bl : forall x y : Char, Char_beq x y = true -> x = y)
+      (Char_lb : forall x y : Char, x = y -> Char_beq x y = true)
+      {T} (G : grammar Char)
+      (Pnil : Prop) ct base v (P2 : _ -> _ -> Prop)
+: forall_reachable_productions
+    G
+    (fun p H => match p with
+                  | [] => Pnil
+                  | x::xs => computes_to
+                               (ct (x::xs))
+                               v
+                             -> P2 x xs
+                end /\ H)
+    True
+  -> forall_reachable_productions
+       G
+       (fun p H => match p with
+                     | [] => Pnil
+                     | x::xs => computes_to
+                                  (forall_reachable_productions
+                                     G
+                                     (fun p0 (else_case : Comp T)
+                                      => if production_beq Char_beq p0 (x::xs)
+                                         then ct p0
+                                         else else_case)
+                                     (base x xs))
+                                  v
+                                -> P2 x xs
+                   end /\ H)
+       True.
+Proof.
+  unfold forall_reachable_productions.
+  repeat (
+      let P := match goal with |- context[fold_right (fun x y => @?P x /\ y) _ _] => constr:P end in
+      pose proof (fold_right_map P and) as H;
+      unfold compose in *; simpl in *;
+      rewrite <- H; clear H
+    ).
+  unfold forall_reachable_productions.
+  match goal with
+    | [ |- _ -> fold_right _ _ (map _ ?ls) ] => induction ls; simpl; trivial; []
+  end.
+  intros [H0 H1]; split; eauto.
+  { match goal with
+      | [ |- match ?e with _ => _ end ] => destruct a; eauto
+    end.
+    match goal with
+      | [ |- context[production_beq _ ?x ?x] ] => rewrite (@production_lb Char Char_beq Char_lb x x eq_refl)
+    end.
+    assumption. }
+  { match goal with
+      | [ H : ?T, H' : ?T -> ?X |- _ ] => specialize (H' H); clear H
+    end.
+    match goal with
+      | [ H : fold_right _ _ (map _ ?ls) |- fold_right _ _ (map _ ?ls) ]
+        => revert H; apply fold_right_and_map_impl; trivial; []
+    end.
+    intros []; trivial; [].
+    intros ??.
+    match goal with
+      | [ |- context[production_beq ?d ?x ?y] ] => case_eq (production_beq d x y); intro
+    end;
+    repeat match goal with
+             | [ H : production_beq _ _ _ = true |- _ ] => apply production_bl in H; [ | assumption.. ]
+             | _ => progress subst
+             | _ => solve [ eauto ]
+           end. }
+Qed.
+
+Lemma exists_in_map_tails {A} (P : _ -> Prop) ls
+: (forall p : list A, (exists prefix, In (prefix ++ p)%list ls) -> P p)
+  <-> fold_right and True (map P (flatten (map tails ls))).
+Proof.
+  induction ls as [ | x xs ]; simpl; split; intros; eauto;
+  try solve [ eauto
+            | destruct_head ex; destruct_head False ].
+  { rewrite map_app, fold_right_app.
+    apply fold_right_and_iff; split.
+    { clear IHxs.
+      specialize (fun p prefix H' => H p (ex_intro _ prefix (or_introl H'))).
+      induction x; simpl; split; try tauto.
+      { apply (H _ []); reflexivity. }
+      { apply (H _ []); reflexivity. }
+      { apply IHx; intros p prefix H'; subst.
+        eapply (H _ (_::prefix)); reflexivity. } }
+    { apply IHxs; intros; destruct_head ex.
+      apply H; eexists; right; eassumption. } }
+  { repeat match goal with
+             | [ H : _ |- _ ] => rewrite map_app in H
+             | [ H : _ |- _ ] => rewrite fold_right_app in H
+             | [ H : fold_right _ ?init _ |- _ ] => not constr_eq init True; apply fold_right_and_iff in H
+             | _ => progress destruct_head_hnf and
+             | _ => progress destruct_head or
+             | _ => progress destruct_head ex
+             | _ => progress subst
+             | _ => progress eauto
+             | [ H : ?T, H' : ?T -> ?X |- _ ] => specialize (H' H)
+           end.
+    let H := match goal with H : fold_right and True (map P (tails (_ ++ ?p))) |- P ?p => constr:H end in
+    clear -H.
+    match goal with
+      | [ H : fold_right and True (map P (tails (?x ++ _))) |- P ?p ] => induction x; destruct p
+    end;
+      simpl in *;
+      destruct_head and; eauto. }
+Qed.
+
+Lemma production_is_reachable__forall_reachable_productions {Char} {G : grammar Char} (P : production Char -> Prop)
+: (forall p, production_is_reachable G p -> P p)
+  <-> (forall_reachable_productions G (fun p H => P p /\ H) True).
+Proof.
+  unfold forall_reachable_productions, production_is_reachable.
+  pose proof (fold_right_map P and) as H; unfold compose in *; simpl in *.
+  rewrite <- H.
+  induction (Valid_nonterminals G) as [ | x xs IHG ]; simpl in *.
+  { split; simpl; intros; trivial.
+    destruct_head ex; destruct_head and; destruct_head False. }
+  { rewrite flatten_app, map_app, fold_right_app.
+    setoid_rewrite fold_right_and_iff.
+    setoid_rewrite <- exists_in_map_tails.
+    setoid_rewrite <- IHG; clear IHG.
+    repeat (split || intro); destruct_head ex; destruct_head and; destruct_head or; subst;
+    match goal with
+      | [ H : _ |- _ ] => apply H
+    end;
+    repeat match goal with
+             | [ |- ex _ ] => eexists
+             | _ => eassumption
+             | [ |- _ /\ _ ] => split; eassumption
+             | [ |- _ /\ _ ] => split; [ left; reflexivity | eassumption ]
+             | [ |- _ /\ _ ] => split; [ right; eassumption | eassumption ]
+           end. }
+Qed.
+
+Lemma production_is_reachable__forall_reachable_productions' {Char} {G : grammar Char} (P : _ -> _ -> Prop)
+: (forall p ps, production_is_reachable G (p::ps) -> P p ps)
+  <-> (forall_reachable_productions G (fun p H => match p with
+                                                    | nil => True
+                                                    | x::xs => P x xs
+                                                  end /\ H) True).
+Proof.
+  setoid_rewrite <- production_is_reachable__forall_reachable_productions.
+  split; intro H.
+  { intros []; intuition. }
+  { intros p ps.
+    specialize (H (p::ps)); eauto. }
+Qed.
+
+Section helpers.
+  Section generic.
+    Context {Char : Type}.
+
+    Fixpoint has_only_terminals (its : production Char)
+    : bool
+      := match its with
+           | nil => true
+           | (Terminal _)::xs => has_only_terminals xs
+           | (NonTerminal _)::_ => false
+         end.
+  End generic.
+
+  Section generic_string.
+    Context {Char} {HSL : StringLike Char} {HLSP : StringLikeProperties Char} (G : grammar Char).
+
+    Lemma has_only_terminals_length {its str}
+          (H0 : @has_only_terminals _ its)
+          (H1 : parse_of_production G str its)
+    : length str = List.length its.
+    Proof.
+      induction H1 as [ | ? ? ? ? pit pits IH ]; simpl in *; trivial.
+      rewrite drop_length in IH.
+      dependent destruction pit.
+      { match goal with
+          | [ H : context[(_ ~= [ _ ])%string_like] |- _ ]
+            => apply length_singleton in H
+        end.
+        rewrite <- IH by assumption; clear IH.
+        repeat match goal with
+                 | _ => intro
+                 | [ H : context[length (take _ _)] |- _ ] => rewrite take_length in H
+                 | [ H : context[length (drop _ _)] |- _ ] => rewrite drop_length in H
+                 | [ H : min ?x ?y = 1 |- _ ] => is_var x; destruct x
+                 | [ H : min (S ?x) ?y = 1 |- _ ] => is_var x; destruct x
+                 | [ H : min (S (S ?x)) ?y = 1 |- _ ] => revert H; apply (Min.min_case_strong (S (S x)) y)
+                 | [ H : context[min _ 0] |- _ ] => rewrite Min.min_0_r in H
+                 | [ H : context[min 0 _] |- _ ] => rewrite Min.min_0_l in H
+                 | [ H : 0 = 1 |- _ ] => exfalso; clear -H; discriminate
+                 | [ H : S (S _) = 1 |- _ ] => exfalso; clear -H; discriminate
+                 | [ H : ?x = 1, H' : context[?x] |- _ ] => rewrite H in H'
+                 | [ H : ?x = 1 |- context[?x] ] => rewrite H
+                 | [ H : min ?x ?y = 1 |- _ ] => revert H; apply (Min.min_case_strong x y)
+                 | _ => omega
+               end. }
+      { exfalso.
+        unfold is_true in *.
+        discriminate. }
+    Qed.
+  End generic_string.
+End helpers.
+
+Section IndexedImpl.
   Context (G : grammar Ascii.ascii).
 
+  Local Notation T := (String.string * (nat * nat))%type (only parsing).
+
+  Local Notation string_of_indexed s :=
+    (substring (fst (snd s)) (snd (snd s)) (fst s))
+      (only parsing).
+  Local Notation ilength s :=
+    (min (String.length (fst s) - fst (snd s)) (snd (snd s)))
+      (only parsing).
+
   Definition expanded_fallback_list
-             (s : (String.string * (nat * nat)))
+             (s : T)
              (it : item Ascii.ascii) (its : production Ascii.ascii)
              (dummy : list nat)
-  : Comp ((String.string * (nat * nat)) * list nat)
+  : Comp (T * list nat)
     := (ls <- (forall_reachable_productions
                  G
                  (fun p else_case
-                  => if production_beq ascii_beq p (it::its)
-                     then (match p return Comp (list nat) with
+                  => If production_beq ascii_beq p (it::its)
+                     Then (match p return Comp (list nat) with
                              | nil => ret dummy
-                             | _::nil => ret [min (String.length (fst s) - fst (snd s)) (snd (snd s))]
+                             | _::nil => ret [ilength s]
                              | (Terminal _):: _ :: _ => ret [1]
                              | (NonTerminal nt):: p'
-                               => if has_only_terminals p'
-                                  then
-                                    ret [min (String.length (fst s) - fst (snd s)) (snd (snd s)) -
-                                         Datatypes.length p']
-                                  else { splits : list nat
+                               => If has_only_terminals p'
+                                  Then
+                                    ret [ilength s - Datatypes.length p']
+                                  Else { splits : list nat
                                        | forall n,
-                                           n <= length (fst s)
-                                           -> parse_of_item G (take n (fst s)) (NonTerminal nt)
-                                           -> parse_of_production G (drop n (fst s)) p'
+                                           n <= ilength s
+                                           -> parse_of_item G (take n (string_of_indexed s)) (NonTerminal nt)
+                                           -> parse_of_production G (drop n (string_of_indexed s)) p'
                                            -> List.In n splits }
                            end)
-                     else else_case)
+                     Else else_case)
                  (ret dummy));
         ret (s, ls))%comp.
 
   Global Arguments expanded_fallback_list / .
 
-  Lemma step_expanded_fallback_list {s p} dummy
-  : refine (fallback_ls <- {ls : list nat |
-                            match fst p with
-                              | Terminal _ => True
-                              | NonTerminal _ =>
-                                if has_only_terminals (snd p)
-                                then True
-                                else
-                                  split_list_is_complete G
-                                                         (substring (fst (snd s))
-                                                                    (snd (snd s)) (fst s))
-                                                         (fst p) (snd p) ls
-                            end};
-            ret
-              (s,
-               match snd p with
-                 | [] => [min (String.length (fst s) - fst (snd s)) (snd (snd s))]
-                 | _ :: _ =>
-                   match fst p with
-                     | Terminal _ => [1]
-                     | NonTerminal _ =>
-                       if has_only_terminals (snd p)
-                       then
-                         [min (String.length (fst s) - fst (snd s)) (snd (snd s)) -
-                          Datatypes.length (snd p)]
-                       else fallback_ls
-                   end
-               end))
-           (expanded_fallback_list s (fst p) (snd p) dummy).
+
+  (** Reference implementation of a [String] that can be split; has a [string], and a start index, and a length *)
+
+  Definition rindexed_spec : ADT (string_rep Ascii.ascii) := ADTRep T {
+    Def Constructor "new"(s : String.string) : rep :=
+      ret (s, (0, String.length s)),
+
+    Def Method "to_string"(s : rep, x : unit) : String.string :=
+      ret (s, string_of_indexed s),
+
+    Def Method "is_char"(s : rep, ch : Ascii.ascii) : bool  :=
+      ret (s, string_beq (string_of_indexed s) (String.String ch "")),
+
+    Def Method "length"(s : rep, x : unit) : nat :=
+      ret (s, ilength s),
+
+    Def Method "take"(s : rep, n : nat) : unit :=
+      ret ((fst s, (fst (snd s), min (snd (snd s)) n)), tt),
+
+    Def Method "drop"(s : rep, n : nat) : unit :=
+      ret ((fst s, (fst (snd s) + n, snd (snd s) - n)), tt),
+
+    Def Method "splits"(s : rep, p : item Ascii.ascii * production Ascii.ascii) : list nat :=
+      dummy <- { ls : list nat | True };
+      expanded_fallback_list s (fst p) (snd p) dummy
+  }.
+
+  Local Ltac fin :=
+    repeat match goal with
+             | _ => progress unfold split_list_is_complete
+             | _ => progress simpl in *
+             | _ => progress computes_to_inv
+             | _ => progress subst
+             | [ |- computes_to (Bind _ _) _ ]
+               => refine ((fun H0 H1 => BindComputes _ _ _ _ H1 H0) _ _)
+             | [ |- computes_to (Return ?x) ?y ]
+               => cut (x = y);
+                 [ let H := fresh in intro H; try rewrite H; eapply ReturnComputes | ]
+             | [ |- computes_to (Pick _) _ ]
+               => eapply PickComputes
+             | _ => reflexivity
+             | _ => assumption
+           end;
+    try solve [ rewrite substring_correct3'; reflexivity
+              | repeat match goal with
+                         | _ => intro
+                         | _ => reflexivity
+                         | _ => rewrite substring_substring
+                         | _ => rewrite Nat.sub_0_r
+                         | _ => rewrite substring_length
+                         | _ => rewrite Nat.add_sub
+                         | _ => rewrite <- Nat.sub_min_distr_r
+                         | _ => progress simpl
+                         | [ |- context[min ?x ?y] ]
+                           => match goal with
+                                | [ |- context[min y x] ]
+                                  => rewrite (Min.min_comm x y)
+                              end
+                         | [ |- context[min (min _ ?x) (?x - ?y)] ]
+                           => rewrite <- (Min.min_assoc _ x (x - y)), (Min.min_r x (x - y)) by omega
+                         | [ |- substring (?x + ?y) _ _ = substring (?y + ?x) _ _ ]
+                           => rewrite (Plus.plus_comm x y)
+                         | [ |- substring ?x ?y ?z = substring ?x (min ?w ?y) ?z ]
+                           => apply (@Min.min_case_strong w y)
+                         | [ H : _ |- _ ] => rewrite Min.min_assoc in H
+                         | _ => apply substring_correct4; omega
+                       end
+              | repeat match goal with
+                         | _ => intro
+                         | _ => progress subst
+                         | [ |- List.In ?x [?y] ] => left
+                         | _ => reflexivity
+                         | [ H : parse_of_production _ _ nil |- _ ] => let H' := fresh in rename H into H'; dependent destruction H'
+                         | [ H : parse_of_production _ _ (_::_) |- _ ] => let H' := fresh in rename H into H'; dependent destruction H'
+                         | [ H : parse_of_item _ _ (Terminal _) |- _ ] => let H' := fresh in rename H into H'; dependent destruction H'
+                         | [ H : parse_of_item _ _ (NonTerminal _) |- _ ] => let H' := fresh in rename H into H'; dependent destruction H'
+                         | _ => erewrite <- has_only_terminals_length by eassumption
+                         | [ H : _ |- _ ] => progress rewrite ?(@drop_length _ string_stringlike string_stringlike_properties), ?(@take_length _ string_stringlike string_stringlike_properties), ?substring_length, ?Nat.add_sub, <- ?plus_n_O, ?Minus.minus_diag, ?Nat.sub_0_r, ?sub_plus in H by omega
+                         | _ => progress rewrite ?drop_length, ?take_length, ?substring_length, ?Nat.add_sub, ?Minus.minus_diag, ?Nat.sub_0_r, <- ?plus_n_O, ?sub_plus by omega
+                         | [ H : is_true (string_beq _ _) |- _ ] => apply string_bl in H
+                         | [ |- _ \/ False ] => left
+                         | [ H : substring _ _ _ = String.String _ _ |- _ = _ :> nat ] => apply (f_equal String.length) in H; simpl in H
+                         | [ H : context[(_ ~= [ _ ])%string_like] |- _ ]
+                           => apply length_singleton in H
+                         | [ |- context[min ?x (?y + ?z) - ?z] ]
+                           => rewrite <- (Nat.sub_min_distr_r x (y + z) z)
+                         | [ H : context[min ?x (?y + ?z) - ?z] |- _ ]
+                           => rewrite <- (Nat.sub_min_distr_r x (y + z) z) in H
+                         | [ H : min ?x ?y = 1 |- _ ] => is_var x; revert H; apply (Min.min_case_strong x y)
+                         | [ H : min ?x ?y = 1 |- _ ] => is_var y; revert H; apply (Min.min_case_strong x y)
+                         | [ H : min ?x ?y = 0 |- _ ] => is_var x; revert H; apply (Min.min_case_strong x y)
+                         | [ H : min ?x ?y = 0 |- _ ] => is_var y; revert H; apply (Min.min_case_strong x y)
+                         | [ H : min ?x 1 = 0 |- _ ] => revert H; apply (Min.min_case_strong x 1)
+                         | [ |- context[0 + ?x] ] => change (0 + x) with x
+                         | [ |- context[?x - S ?y] ]
+                           => not constr_eq y 0; rewrite !(Nat.sub_succ_r x y), !Minus.pred_of_minus
+                         | [ H : ?x = 1 |- context[?x] ] => rewrite H
+                         | [ H : ?x = 1, H' : context[?x] |- _ ] => rewrite H in H'
+                         | [ H : ?x <= ?y |- context[?x - ?y] ] => replace (x - y) with 0 by (clear -H; omega)
+                         | [ H : context[?x - ?y], H' : ?x <= ?y |- _ ]
+                           => rewrite (proj2 (@Nat.sub_0_le x y)) in H by exact H'
+                         | [ H : context[min 0 ?x] |- _ ] => change (min 0 x) with 0 in H
+                         | [ |- 1 = ?x ] => is_var x; destruct x
+                         | [ |- 1 = S ?x ] => is_var x; destruct x
+                         | [ H : _ <= 0 |- _ ] => apply Le.le_n_0_eq in H; symmetry in H
+                         | [ H : context[min 1 ?x] |- _ ] => is_var x; destruct x
+                         | [ H : context[min 1 (S ?x)] |- _ ] => is_var x; destruct x
+                         | [ H : context[min 1 (S ?x)] |- _ ] => change (min 1 (S x)) with 1 in H
+                         | [ H : context[min ?x ?y], H' : ?x <= ?y |- _ ] => rewrite Min.min_l in H by assumption
+                         | [ H : context[min ?x ?y], H' : ?y <= ?x |- _ ] => rewrite Min.min_r in H by assumption
+                         | [ H : context[min (?x - ?y) ?x] |- _ ] => rewrite Min.min_l in H by omega
+                         | [ H : context[min ?x (?x - ?y)] |- _ ] => rewrite Min.min_r in H by omega
+                         | _ => omega
+                       end ].
+
+  Lemma FirstStep
+  : refineADT (string_spec G) rindexed_spec.
   Proof.
-    unfold expanded_fallback_list, forall_reachable_productions, split_list_is_complete, production_is_reachable.
-    generalize (Valid_nonterminals G).
-    intro ls; revert p; induction ls.
-    { simpl.
-      repeat intro; computes_to_inv; subst.
-      destruct (fst p); simpl.
-      {
-    intro ls; induction ls
-    simplify with monad laws.
+    econstructor 1 with (AbsR := (fun r_o r_n =>
+                                    substring (fst (snd r_n)) (snd (snd r_n)) (fst r_n) = r_o));
 
-{ls : list nat |
-                     match fst n with
-                     | Terminal _ => True
-                     | NonTerminal _ =>
-                         if has_only_terminals (snd n)
-                         then True
-                         else
-                          split_list_is_complete G
-                            (substring (fst (snd r_n))
-                               (snd (snd r_n)) (fst r_n))
-                            (fst n) (snd n) ls
-                     end}
-
-
-  (** A production is reachable if it is the tail of a production
-      associated to a valid nonterminal. *)
-  Definition production_is_reachable (p : production Char) : Prop
-    := exists nt prefix,
-         List.In nt (Valid_nonterminals G)
-         /\ List.In
-              (prefix ++ p)
-              (Lookup G nt).
-
-  (** A list of splits is complete if, for every reachable production,
-      it contains every index of the string that yields a parse tree
-      for that production by splitting at that index. *)
-  Definition split_list_is_complete `{HSL : StringLike Char} (str : String) (it : item Char) (its : production Char)
-             (splits : list nat)
-  : Prop
-    := forall n,
-         n <= length str
-         -> parse_of_item G (take n str) it
-         -> parse_of_production G (drop n str) its
-         -> production_is_reachable (it::its)
-         -> List.In n splits.
-
-  Record Splitter :=
-    {
-      string_type :> StringLike Char;
-      splits_for : String -> item Char -> production Char -> list nat;
-      (** give a list of indices for splitting a given string *)
-
-      string_type_properties :> StringLikeProperties Char;
-      splits_for_complete : forall str it its,
-                              split_list_is_complete str it its (splits_for str it its)
-      (** [splits_for] must contain all valid indices for splitting *)
-    }.
-
-  Global Existing Instance string_type.
-  Global Existing Instance string_type_properties.
-
-  Record Parser (splitter : Splitter) :=
-    {
-      has_parse : @String Char splitter -> bool;
-      (** does this string parse as the start symbol of the grammar? *)
-
-      has_parse_sound : forall str,
-                          has_parse str = true
-                          -> parse_of_item G str (NonTerminal (Start_symbol G));
-
-      has_parse_complete : forall str (p : parse_of_item G str (NonTerminal (Start_symbol G))),
-                             Forall_parse_of_item
-                               (fun _ nt => List.In nt (Valid_nonterminals G))
-                               p
-                             -> has_parse str = true
-    }.
-End interface.
+        eapply Iterate_Ensemble_BoundedIndex_equiv;
+        simpl; intuition; intros; try simplify with monad laws;
+        repeat intro; computes_to_inv; subst; simpl;
+        fin.
+    { intros.
+      match goal with
+        | [ H' : appcontext[forall_reachable_productions], H : production_is_reachable G (?x::?xs) |- _ ]
+          => move H' at top; move H at top; generalize dependent xs; intros xs H H';
+             move H' at top; move H at top; generalize dependent x; intros x H; revert x xs H
+      end.
+      refine (proj2 (@production_is_reachable__forall_reachable_productions' Ascii.ascii G _) _).
+      apply (forall_reachable_productions_helper (@ascii_bl) (@ascii_lb)).
+      unfold forall_reachable_productions.
+      lazymatch goal with
+        | [ |- context[fold_right (fun x y => @?P x /\ y) _ _] ]
+          => let H' := fresh in
+             pose proof (fold_right_map P and) as H';
+               unfold compose in H'; simpl in H';
+               rewrite <- H'; clear H'
+      end.
+      generalize (flatten
+                    (flatten
+                       (map (fun nt : string => map tails (G nt))
+                            (Valid_nonterminals G)))).
+      intro ls; induction ls; simpl; trivial; [].
+      { repeat match goal with
+                 | [ |- _ /\ _ ] => split
+                 | [ |- context[match ?e with _ => _ end] ] => atomic e; destruct e
+                 | [ |- context[production_beq _ ?x ?x] ] => rewrite (production_lb (@ascii_lb) eq_refl)
+                 | _ => solve [ trivial ]
+               end.
+        { clear IHls; intros; abstract fin. }
+        { clear IHls; intros; abstract fin. }
+        { clear IHls; intros; abstract fin. }
+        { clear IHls; unfold If_Then_Else.
+          abstract (
+              repeat match goal with
+                       | _ => intro
+                       | [ H : context[if has_only_terminals ?e then _ else _] |- _ ]
+                         => (revert H; case_eq (has_only_terminals e))
+                       | _ => progress computes_to_inv
+                       | _ => progress subst
+                       | [ |- In _ [_] ] => left
+                       | _ => erewrite <- has_only_terminals_length by eassumption
+                       | [ H : _ |- _ ] => progress rewrite ?substring_length, ?Nat.add_sub in H
+                       | _ => progress rewrite ?substring_length, ?Nat.add_sub
+                       | [ |- context[min ?x (?y + ?z) - ?z] ]
+                         => rewrite <- (Nat.sub_min_distr_r x (y + z) z)
+                       | [ H : context[min ?x (?y + ?z) - ?z] |- _ ]
+                         => rewrite <- (Nat.sub_min_distr_r x (y + z) z) in H
+                       | [ |- context[min (?x - ?y) ?x] ] => rewrite (Min.min_l (x - y) x) by omega
+                       | [ |- context[min ?x (?x - ?y)] ] => rewrite (Min.min_r x (x - y)) by omega
+                       | _ => omega
+                       | _ => solve [ eauto ]
+                     end
+            ). } } }
+  Qed.
+End IndexedImpl.
