src/Parsers/Refinement/SharpenedABStar.v
@@ -1,0 +1,119 @@
+(** Sharpened ADT for (ab)* *)
+Require Import ADTSynthesis.Parsers.Refinement.Tactics.
+Require Import ADTSynthesis.Parsers.Grammars.ABStar.
+Set Implicit Arguments.
+
+Section IndexedImpl.
+
+  Lemma ComputationalSplitter
+  : FullySharpened (string_spec ab_star_grammar).
+  Proof.
+    start honing parser using indexed representation.
+
+    hone method "splits".
+    {
+      simplify parser splitter.
+      finish honing parser method.
+    }
+
+    FullySharpenEachMethodWithoutDelegation.
+    extract delegate-free implementation.
+  Defined.
+
+End IndexedImpl.
+
+Require Import ADTSynthesis.Parsers.ParserFromParserADT.
+
+Local Ltac do_compute_in term hyp :=
+  let term' := (eval compute in term) in
+  change term with term' in hyp.
+
+Local Ltac do_lazy_in term hyp :=
+  let term' := (eval lazy in term) in
+  change term with term' in hyp.
+
+Local Ltac do_simpl_in term hyp :=
+  let term' := (eval simpl in term) in
+  change term with term' in hyp.
+
+Local Arguments string_dec : simpl never.
+Local Arguments Equality.string_beq : simpl never.
+Local Notation hextr0 := (ex _).
+Local Notation exist' x := (exist _ x _).
+Local Notation hextr1 := (or_intror _).
+Local Notation hextr2 := (or_introl _).
+
+Definition ab_star_parser' (str : String.string) : bool.
+Proof.
+  pose (string_has_parse ComputationalSplitter str) as impl.
+  cbv beta iota zeta delta [string_has_parse ParserInterface.has_parse base_parser ParserImplementation.parser BooleanRecognizer.parse_nonterminal BooleanRecognizer.parse_nonterminal_or_abort BooleanRecognizer.parse_nonterminal_step BooleanRecognizer.parse_productions BaseTypes.initial_nonterminals_data BooleanBaseTypes.predata ParserImplementation.parser_data RDPList.rdp_list_predata BaseTypes.remove_nonterminal BaseTypes.nonterminals_listT_R BaseTypes.nonterminals_listT RDPList.rdp_list_nonterminals_listT RDPList.rdp_list_nonterminals_listT_R BaseTypes.is_valid_nonterminal RDPList.rdp_list_is_valid_nonterminal BaseTypes.ntl_wf RDPList.rdp_list_remove_nonterminal] in impl.
+  change (@StringLike.String Ascii.ascii (ParserInterface.string_type
+                                            (SplitterFromParserADT.adt_based_splitter
+                                               ComputationalSplitter)))
+  with ({ r : (String.string * (nat * nat)) | exists orig, AbsR (projT2 ComputationalSplitter) orig r }%type)
+    in impl.
+  Timeout 2 change ((@StringLike.length _ (ParserInterface.string_type
+                                             (SplitterFromParserADT.adt_based_splitter
+                                                ComputationalSplitter))))
+  with (fun str : { r : (String.string * (nat * nat)) | exists orig, AbsR (projT2 ComputationalSplitter) orig r }%type => ilength (` str)).
+  do_simpl_in (Valid_nonterminals ab_star_grammar) impl.
+  Timeout 2 change (new_string_of_base_string ComputationalSplitter str)
+  with (exist _ (str, (0, String.length str)) (proj2_sig (new_string_of_base_string ComputationalSplitter str))) in impl.
+  Arguments new_string_of_base_string / .
+
+  Timeout 2 do_simpl_in (new_string_of_base_string ComputationalSplitter str) impl.
+
+  Timeout 2 do_simpl_in (@StringLike.length _ (ParserInterface.string_type
+                                                (SplitterFromParserADT.adt_based_splitter
+                                                   ComputationalSplitter))) impl.
+  Timeout 2 lazy beta iota zeta delta [BaseTypes.remove_nonterminal BaseTypes.nonterminals_listT_R StringLike.String StringLike.length] in impl.
+  unfold Lookup in *.
+
+  unfold RelationClasses.reflexivity in impl.
+  unfold RelationClasses.Equivalence_Reflexive in impl.
+  unfold bool_eq_Equivalence in *.
+  Timeout 3 cbv delta [BooleanRecognizer.parse_nonterminal BooleanRecognizer.parse_nonterminal_or_abort] in b.
+  Timeout 10 simpl in b.
+  let impl := (eval unfold b in b) in
+  let impl' := (eval cbv beta iota zeta delta [BooleanRecognizer.parse_nonterminal] in impl) in
+  pose impl'.
+Timeout 2 simpl in b.
+  refine (fun s => has_parse (parser (adt_based_splitter ComputationalSplitter))
+                             (exist _ (cConstructors (projT1 ComputationalSplitter) {| StringBound.bindex := "new" |} s) (ex_intro _ s _))).
+  abstract (
+      pose proof (ADTRefinementPreservesConstructors (projT2 ComputationalSplitter) {| StringBound.bindex := "new" |} s (cConstructors (projT1 ComputationalSplitter) {| StringBound.bindex := "new" |} s) (ReturnComputes _)) as H'';
+      computes_to_inv;
+      simpl in H'';
+      computes_to_inv; subst; assumption
+    ).
+Defined.
+
+Definition ab_star_parser' : String.string -> bool.
+Proof.
+Print ab_star_parser.
+
+
+  hnf.
+  simpl.
+  simpl.
+  pose .
+  simpl in *.
+  Require Import StringLike.Core StringLike.String.
+  Timeout 2 simpl.
+  hnf.
+  unfold string_type.
+  Locate adt_based_splitter.
+  pose .
+  simpl in c.
+  unfold cConstructorType in *.
+
+lazy.
+ (s, (0, String.length s))).
+    simpl in b.
+Require Import StringLike.Core.
+simpl in b.
+Set Printing All.
+
+
+Check ab_star_parser.
+Check .
